@prefix : <http://purl.org/query/voidext#> .
@prefix owl: <http://www.w3.org/2002/07/owl#> .
@prefix rdf: <http://www.w3.org/1999/02/22-rdf-syntax-ns#> .
@prefix xml: <http://www.w3.org/XML/1998/namespace> .
@prefix xsd: <http://www.w3.org/2001/XMLSchema#> .
@prefix rdfs: <http://www.w3.org/2000/01/rdf-schema#> .
@base <http://purl.org/voidext> .

<http://purl.org/voidext> rdf:type owl:Ontology ;
                           owl:versionInfo "The Extension of the Vocabulary of Interlinked Datasets (VoID) RDF Schema to include the concept of virtual links. Author: Tarcisio Mendes de Farias"@en .

#################################################################
#    Annotation properties
#################################################################

###  http://rdfs.org/ns/void#dataDump
<http://rdfs.org/ns/void#dataDump> rdfs:comment "An RDF dump, partial or complete, of a void:Dataset."@en ;
                                   rdfs:label "data dump"@en ;
                                   rdf:type owl:AnnotationProperty ;
                                   rdfs:domain <http://rdfs.org/ns/void#Dataset> .


###  http://rdfs.org/ns/void#rootResource
<http://rdfs.org/ns/void#rootResource> rdfs:comment "A top concept or entry point for a void:Dataset that is structured in a tree-like fashion. All resources in a dataset can be reached by following links from its root resources in a small number of steps." ;
                                       rdfs:label "root resource" ;
                                       rdf:type owl:AnnotationProperty ;
                                       rdfs:domain <http://rdfs.org/ns/void#Dataset> .


###  http://rdfs.org/ns/void#sparqlEndpoint
<http://rdfs.org/ns/void#sparqlEndpoint> rdfs:label "has a SPARQL endpoint at" ;
                                         rdf:type owl:AnnotationProperty ;
                                         rdfs:domain <http://rdfs.org/ns/void#Dataset> .


###  http://rdfs.org/ns/void#uriLookupEndpoint
<http://rdfs.org/ns/void#uriLookupEndpoint> rdfs:comment "Defines a simple URI look-up protocol for accessing a dataset." ;
                                            rdfs:label "has an URI look-up endpoint at" ;
                                            rdf:type owl:AnnotationProperty ;
                                            rdfs:domain <http://rdfs.org/ns/void#Dataset> .


###  http://rdfs.org/ns/void#uriRegexPattern
<http://rdfs.org/ns/void#uriRegexPattern> rdfs:comment "Defines a regular expression pattern matching URIs in the dataset." ;
                                          rdfs:label "has URI regular expression pattern" ;
                                          rdf:type owl:AnnotationProperty ;
                                          rdfs:domain <http://rdfs.org/ns/void#Dataset> .


###  http://rdfs.org/ns/void#vocabulary
<http://rdfs.org/ns/void#vocabulary> rdfs:comment "A vocabulary that is used in the dataset." ;
                                     rdfs:label "vocabulary" ;
                                     rdf:type owl:AnnotationProperty ;
                                     rdfs:domain <http://rdfs.org/ns/void#Dataset> .


#################################################################
#    Object Properties
#################################################################

###  http://purl.org/query/voidext#intersectAt
:intersectAt rdf:type owl:ObjectProperty ;
             rdfs:domain :ComplexLinkSet ;
             rdfs:range <http://rdfs.org/ns/void#Linkset> ;
             rdfs:comment "This property assings exactly two void:LinkSet(s) to compose a complex link set. For each void:LinkSet, either the subject or the object node of one link predicate intersects the another one. It means that the subject or object of a link predicate is exactly the same as the another link predicate. However, these predicates are stored in different void:datasets."@en ;
             rdfs:label "intersects at"@en .


###  http://purl.org/query/voidext#intersectionType
:intersectionType rdf:type owl:ObjectProperty ;
                  rdfs:domain :ComplexLinkSet ;
                  rdfs:range :LinkSetIntersection ;
                  rdfs:comment "This property assings the intersection type of the graph nodes in different void:Dataset(s) (i.e. either the subject or the object node of a link predicate)."@en ;
                  rdfs:label "intersection type"@en .


###  http://purl.org/query/voidext#linkPredicateDomain
:linkPredicateDomain rdf:type owl:ObjectProperty ;
                     rdfs:domain <http://rdfs.org/ns/void#Linkset> ;
                     rdfs:range rdfs:Class ;
                     rdfs:comment "the link predicate subject type if specified (i.e. relation domain)."@en ;
                     rdfs:label "link predicate domain"@en .


###  http://purl.org/query/voidext#linkPredicateRange
:linkPredicateRange rdf:type owl:ObjectProperty ;
                    rdfs:domain <http://rdfs.org/ns/void#Linkset> ;
                    rdfs:range rdfs:Class ;
                    rdfs:comment "the link predicate object type if specified (i.e. relation range)."@en ;
                    rdfs:label "link predicate range"@en .


###  http://purl.org/query/voidext#sharedInstanceType
:sharedInstanceType rdf:type owl:ObjectProperty ;
                    rdfs:domain :SharedInstanceSet ;
                    rdfs:range rdfs:Class ,
                               owl:Class ;
                    rdfs:comment "This property assings the type (i.e. a common class) of the shared instances between two different void:Dataset(s). Shared instances implies the same IRI however stored in different data stores."@en ;
                    rdfs:label "shared instance type"@en .


###  http://rdfs.org/ns/void#class
<http://rdfs.org/ns/void#class> rdf:type owl:ObjectProperty ;
                                rdfs:domain <http://rdfs.org/ns/void#Dataset> ;
                                rdfs:range rdfs:Class ;
                                rdfs:comment "The rdfs:Class that is the rdf:type of all entities in a class-based partition." ;
                                rdfs:label "class" .


###  http://rdfs.org/ns/void#classPartition
<http://rdfs.org/ns/void#classPartition> rdf:type owl:ObjectProperty ;
                                         rdfs:subPropertyOf <http://rdfs.org/ns/void#subset> ;
                                         rdfs:domain <http://rdfs.org/ns/void#Dataset> ;
                                         rdfs:range <http://rdfs.org/ns/void#Dataset> ;
                                         rdfs:comment "A subset of a void:Dataset that contains only the entities of a certain rdfs:Class." ;
                                         rdfs:label "class partition" .


###  http://rdfs.org/ns/void#exampleResource
<http://rdfs.org/ns/void#exampleResource> rdf:type owl:ObjectProperty ;
                                          rdfs:domain <http://rdfs.org/ns/void#Dataset> ;
                                          rdfs:range rdfs:Resource ;
                                          rdfs:label "example resource of dataset" .


###  http://rdfs.org/ns/void#feature
<http://rdfs.org/ns/void#feature> rdf:type owl:ObjectProperty ;
                                  rdfs:domain <http://rdfs.org/ns/void#Dataset> ;
                                  rdfs:range <http://rdfs.org/ns/void#TechnicalFeature> ;
                                  rdfs:comment "A void:TechnicalFeature supported by a void:Datset."@en ;
                                  rdfs:label "feature"@en .


###  http://rdfs.org/ns/void#inDataset
<http://rdfs.org/ns/void#inDataset> rdf:type owl:ObjectProperty ;
                                    rdfs:domain <http://xmlns.com/foaf/0.1/Document> ;
                                    rdfs:range <http://rdfs.org/ns/void#Dataset> ;
                                    rdfs:comment "Points to the void:Dataset that a document is a part of." ;
                                    rdfs:label "in dataset" .


###  http://rdfs.org/ns/void#linkPredicate
<http://rdfs.org/ns/void#linkPredicate> rdf:type owl:ObjectProperty ;
                                        rdfs:domain <http://rdfs.org/ns/void#Linkset> ;
                                        rdfs:range rdf:Property ;
                                        rdfs:label "a link predicate" .


###  http://rdfs.org/ns/void#objectsTarget
<http://rdfs.org/ns/void#objectsTarget> rdf:type owl:ObjectProperty ;
                                        rdfs:subPropertyOf <http://rdfs.org/ns/void#target> ;
                                        rdfs:domain <http://rdfs.org/ns/void#Linkset> ;
                                        rdfs:range <http://rdfs.org/ns/void#Dataset> ;
                                        rdfs:comment "The dataset describing the objects of the triples contained in the Linkset." ;
                                        rdfs:label "objects target" .


###  http://rdfs.org/ns/void#openSearchDescription
<http://rdfs.org/ns/void#openSearchDescription> rdf:type owl:ObjectProperty ;
                                                rdfs:domain <http://rdfs.org/ns/void#Dataset> ;
                                                rdfs:range <http://xmlns.com/foaf/0.1/Document> ;
                                                rdfs:comment "An OpenSearch description document for a free-text search service over a void:Dataset." ;
                                                rdfs:label "open search description" .


###  http://rdfs.org/ns/void#property
<http://rdfs.org/ns/void#property> rdf:type owl:ObjectProperty ;
                                   rdfs:domain <http://rdfs.org/ns/void#Dataset> ;
                                   rdfs:range rdf:Property ;
                                   rdfs:comment "The rdf:Property that is the predicate of all triples in a property-based partition." ;
                                   rdfs:label "property" .


###  http://rdfs.org/ns/void#propertyPartition
<http://rdfs.org/ns/void#propertyPartition> rdf:type owl:ObjectProperty ;
                                            rdfs:subPropertyOf <http://rdfs.org/ns/void#subset> ;
                                            rdfs:domain <http://rdfs.org/ns/void#Dataset> ;
                                            rdfs:range <http://rdfs.org/ns/void#Dataset> ;
                                            rdfs:comment "A subset of a void:Dataset that contains only the triples of a certain rdf:Property." ;
                                            rdfs:label "property partition" .


###  http://rdfs.org/ns/void#subjectsTarget
<http://rdfs.org/ns/void#subjectsTarget> rdf:type owl:ObjectProperty ;
                                         rdfs:subPropertyOf <http://rdfs.org/ns/void#target> ;
                                         rdfs:domain <http://rdfs.org/ns/void#Linkset> ;
                                         rdfs:range <http://rdfs.org/ns/void#Dataset> ;
                                         rdfs:comment "The dataset describing the subjects of triples contained in the Linkset." ;
                                         rdfs:label "subjects target" .


###  http://rdfs.org/ns/void#subset
<http://rdfs.org/ns/void#subset> rdf:type owl:ObjectProperty ;
                                 rdfs:domain <http://rdfs.org/ns/void#Dataset> ;
                                 rdfs:range <http://rdfs.org/ns/void#Dataset> ;
                                 rdfs:label "has subset" .


###  http://rdfs.org/ns/void#target
<http://rdfs.org/ns/void#target> rdf:type owl:ObjectProperty ;
                                 rdfs:domain <http://rdfs.org/ns/void#Linkset> ;
                                 rdfs:range <http://rdfs.org/ns/void#Dataset> ;
                                 rdfs:comment "One of the two datasets linked by the Linkset." ;
                                 rdfs:label "target" .


#################################################################
#    Data properties
#################################################################

###  http://rdfs.org/ns/void#distinctObjects
<http://rdfs.org/ns/void#distinctObjects> rdf:type owl:DatatypeProperty ;
                                          rdfs:domain <http://rdfs.org/ns/void#Dataset> ;
                                          rdfs:range xsd:integer ;
                                          rdfs:comment "The total number of distinct subjects in the dataset. In other words, the number of distinct URIs or blank nodes that occur in the subject position of triples in the dataset."@en ;
                                          rdfs:label "number of distinct objects"@en .


###  http://rdfs.org/ns/void#distinctSubjects
<http://rdfs.org/ns/void#distinctSubjects> rdf:type owl:DatatypeProperty ;
                                           rdfs:domain <http://rdfs.org/ns/void#Dataset> ;
                                           rdfs:range xsd:integer ;
                                           rdfs:comment "The total number of distinct objects in the dataset. In other words, the number of distinct URIs, blank nodes, or literals that occur in the object position of triples in the dataset."@en ;
                                           rdfs:label "number of distinct subjects"@en .


###  http://rdfs.org/ns/void#documents
<http://rdfs.org/ns/void#documents> rdf:type owl:DatatypeProperty ;
                                    rdfs:domain <http://rdfs.org/ns/void#Dataset> ;
                                    rdfs:range xsd:integer ;
                                    rdfs:comment "If the dataset is published as a set of individual documents, such as RDF/XML documents or RDFa-annotated web pages, then this property indicates the total number of such documents. Non-RDF documents, such as web pages in HTML or images, are usually not included in this count. This property is intended for datasets where the total number of triples or entities is hard to determine. void:triples or void:entities should be preferred where practical."@en ;
                                    rdfs:label "number of documents"@en .


###  http://rdfs.org/ns/void#entities
<http://rdfs.org/ns/void#entities> rdf:type owl:DatatypeProperty ;
                                   rdfs:domain <http://rdfs.org/ns/void#Dataset> ;
                                   rdfs:range xsd:integer ;
                                   rdfs:comment "The total number of entities that are described in the dataset. To be an entity in a dataset, a resource must have a URI, and the URI must match the dataset's void:uriRegexPattern, if any. Authors of VoID files may impose arbitrary additional requirements, for example, they may consider any foaf:Document resources as not being entities."@en ;
                                   rdfs:label "number of entities"@en .


###  http://rdfs.org/ns/void#properties
<http://rdfs.org/ns/void#properties> rdf:type owl:DatatypeProperty ;
                                     rdfs:domain <http://rdfs.org/ns/void#Dataset> ;
                                     rdfs:range xsd:integer ;
                                     rdfs:comment "The total number of distinct properties in a void:Dataset. In other words, the number of distinct resources that occur in the predicate position of triples in the dataset." ;
                                     rdfs:label "number of properties" .


###  http://rdfs.org/ns/void#triples
<http://rdfs.org/ns/void#triples> rdf:type owl:DatatypeProperty ;
                                  rdfs:domain <http://rdfs.org/ns/void#Dataset> ;
                                  rdfs:range xsd:integer ;
                                  rdfs:comment "The total number of triples contained in a void:Dataset."@en ;
                                  rdfs:label "number of triples"@en .


###  http://rdfs.org/ns/void#uriSpace
<http://rdfs.org/ns/void#uriSpace> rdf:type owl:DatatypeProperty ;
                                   rdfs:domain <http://rdfs.org/ns/void#Dataset> ;
                                   rdfs:range rdfs:Literal ;
                                   rdfs:comment "A URI that is a common string prefix of all the entity URIs in a void:Dataset." ;
                                   rdfs:label "URI space" .


#################################################################
#    Classes
#################################################################

###  http://purl.org/query/voidext#ComplexLinkSet
:ComplexLinkSet rdf:type owl:Class ;
                rdfs:subClassOf :VirtualLinks ;
                rdfs:comment "It contains exactly two void:LinkSet(s) to compose a complex link set. Two link sets that intersects at some graph node (e.g. the object nodes of link predicates)"@en ;
                rdfs:label "Complex link set"@en .


###  http://purl.org/query/voidext#LinkSetIntersection
:LinkSetIntersection rdf:type owl:Class ;
                     rdfs:comment "The possible intersection types between the graph nodes in different void:Dataset(s) (i.e. either the subject or the object node of a link predicate). The instances of this class are exclusively voidext:OBJECT_OBJECT, voidext:OBJECT_SUBJECT, and voidext:SUBJECT_SUBJECT."@en ;
                     rdfs:label "Link set intersection"@en .


###  http://purl.org/query/voidext#SharedInstanceSet
:SharedInstanceSet rdf:type owl:Class ;
                   rdfs:subClassOf :VirtualLinks ;
                   rdfs:comment "Shared IRI instances usually of the same OWL/RDFS class which are stored in two or more different void:Dataset(s)."@en ;
                   rdfs:label "Shared instance set"@en .


###  http://purl.org/query/voidext#VirtualLinks
:VirtualLinks rdf:type owl:Class ;
              rdfs:subClassOf <http://rdfs.org/ns/void#Dataset> ;
              rdfs:comment "A virtual link is an intersection data point between two or more void:Dataset(s) that is not concretely stored. The link is established during the federated or distributed query execution."@en ;
              rdfs:label "Virtual link set"@en .


###  http://rdfs.org/ns/void#Dataset
<http://rdfs.org/ns/void#Dataset> rdf:type owl:Class ;
                                  rdfs:comment "A set of RDF triples that are published, maintained or aggregated by a single provider." ;
                                  rdfs:label "dataset" .


###  http://rdfs.org/ns/void#DatasetDescription
<http://rdfs.org/ns/void#DatasetDescription> rdf:type owl:Class ;
                                             rdfs:subClassOf <http://xmlns.com/foaf/0.1/Document> ;
                                             rdfs:comment "A web resource whose foaf:primaryTopic or foaf:topics include void:Datasets." ;
                                             rdfs:label "dataset description" .


###  http://rdfs.org/ns/void#Linkset
<http://rdfs.org/ns/void#Linkset> rdf:type owl:Class ;
                                  rdfs:subClassOf :VirtualLinks ;
                                  rdfs:comment "A collection of RDF links between two void:Datasets." ;
                                  rdfs:label "Link set" .


###  http://rdfs.org/ns/void#TechnicalFeature
<http://rdfs.org/ns/void#TechnicalFeature> rdf:type owl:Class ;
                                           rdfs:comment "A technical feature of a void:Dataset, such as a supported RDF serialization format." ;
                                           rdfs:label "technical feature" .


###  http://www.w3.org/1999/02/22-rdf-syntax-ns#Property
rdf:Property rdf:type owl:Class .


###  http://www.w3.org/2000/01/rdf-schema#Class
rdfs:Class rdf:type owl:Class .


###  http://www.w3.org/2000/01/rdf-schema#Resource
rdfs:Resource rdf:type owl:Class .


###  http://www.w3.org/2002/07/owl#Class
owl:Class rdf:type owl:Class .


###  http://xmlns.com/foaf/0.1/Document
<http://xmlns.com/foaf/0.1/Document> rdf:type owl:Class .


#################################################################
#    Individuals
#################################################################

###  http://purl.org/query/voidext#OBJECT_OBJECT
:OBJECT_OBJECT rdf:type owl:NamedIndividual ,
                        :LinkSetIntersection ;
               rdfs:comment "The intersection between two void:Dataset(s) (i.e. knowledge graphs) occurs at the object node in both data sets."@en ;
               rdfs:label "Object - Object intersection"@en .


###  http://purl.org/query/voidext#SUBJECT_OBJECT
:SUBJECT_OBJECT rdf:type owl:NamedIndividual ,
                         :LinkSetIntersection ;
                rdfs:comment "The intersection between two void:Dataset(s) (i.e. knowledge graphs) occurs at the object node of one data set (graph) and the subject node of another data set (graph)."@en ;
                rdfs:label "Subject - Object intersection"@en .


###  http://purl.org/query/voidext#SUBJECT_SUBJECT
:SUBJECT_SUBJECT rdf:type owl:NamedIndividual ,
                          :LinkSetIntersection ;
                 rdfs:comment "The intersection between two void:Dataset(s) (i.e. knowledge graphs) occurs at the subject node in both data sets."@en ;
                 rdfs:label "Subject - Subject intersection"@en .


###  Generated by the OWL API (version 5.1.7) https://github.com/owlcs/owlapi/
